#+STARTUP: overview
#+TITLE: Lessong 1
#+CREATOR: Andriy
#+ 
* Heading 
Sample text

** More text
** Lower Level Heading
* 


#+BEGIN_SRC emacs-lisp

#+END_SRC



Assignment 1
3FP3
McMaster University
Andriy Yuzva
yuzvaa@mcmaster.ca

\begin{code}
module Assignment_1 where
\end{code}

\begin{code}
--------------------Qustion 1--------------------
matches :: Eq a => a -> [a] -> [a]
matches given []       = []
matches given (first : rest) | (given == first) = given : given `matches` rest
                             | otherwise = given `matches` rest
                             
elem' :: Eq a => a -> [a] -> Bool
elem' given [] = False
elem' given (first : rest) | (given == first) = True
                          | otherwise = elem' given rest

assignPos :: Eq a => Integer -> a -> [a] -> [Integer]
assignPos _ given [] = []
assignPos position given (current : rest) | given == current = position : assignPos (position + 1) given rest
                                        | otherwise        = assignPos (position + 1) given rest

pos :: Eq a => a -> [a] -> [Integer]
pos given [] = [ -1 ]
pos given sequence = assignPos 0 given sequence
\end{code}

Out of the three functions, the first two are best. I believe that because these functions 
are implemented within themselves and do not rely on helper functions. Pos could be implemented 
via zip filter and map, in which case helper would not be required. Alternatively, if pos requirment
was modified to also take current index as argument it would not need helper.

\begin{code}
--------------------Qustion 2--------------------

applyAll :: [a -> b] -> [a] -> [b]
applyAll [] values = []
applyAll functions [] = []
applyAll (function : remainingFunct) values = (function `map` values) ++ (applyAll remainingFunct values)

\end{code}

\begin{code}
--------------------Qustion 3--------------------
--Using explicit recursion
tripleNeg1 :: (Ord a, Num a) => [a] -> [a]
tripleNeg1 [] = []
tripleNeg1 (value : rest) | value >= 0  = value : tripleNeg1 rest
                          | otherwise = 3 * value : tripleNeg1 rest

tripleNeg2Decorator :: (Ord a, Num a) => [a] -> [Either a a]
tripleNeg2Decorator [] = []
tripleNeg2Decorator values = map (\x -> if (x >= 0) then Right(x) else Left(x)) values

--Using Haskell either and map
tripleNeg2 :: (Ord a, Num a) => [a] -> [a]
tripleNeg2 [] = []
tripleNeg2 values = (either (3*) (1*)) `map` tripleNeg2Decorator(values)

\end{code}

\begin{code}
--------------------Qustion 4--------------------
data OrBoth a b  = Left' a | Right' b | Both a b

consume1 :: (a -> c) -> (b -> c) -> (a -> b -> c) -> OrBoth a b -> c
consume1 f _ _ (Left' x) = f x
consume1 _ f _ (Right' x) = f x
consume1 _ _ f (Both x y) = f x y

consume2 :: (a -> c) -> (b -> c) -> (c -> c -> c) -> OrBoth a b -> c
consume2 f _ _ (Left' x) = f x
consume2 _ f _ (Right' x) = f x
consume2 fl fr f (Both x y) = f (fl x) (fr y)

\end{code}

I believe consume1 is better. It has 3 separate functions applied only once.
This scenario occurs more frequently in practice than having to apply both 
functions, as well as the 'Both' case function on top.

\begin{code}
--------------------Qustion 5--------------------
data Ternary a = TLeaf a | TNode (Ternary a) (Ternary a) (Ternary a)

mirror :: Ternary a -> Ternary a
mirror (TLeaf a) = (TLeaf a) 
mirror (TNode child1 child2 child3) = (TNode child3 child2 child1)

flattenTernary :: Ternary a -> [a]
flattenTernary (TLeaf a) = [a] 
flattenTernary (TNode child1 child2 child3) = (flattenTernary child1) ++ (flattenTernary child2) ++ (flattenTernary child3)
\end{code}

\begin{code}
--------------------Qustion 6--------------------
--Given:
all' :: (a -> Bool) -> [a] -> Bool 
all' p [] = True 
all' p (x : xs) = p x && (all' p xs)
\end{code}
Prove:
    ∀p, xs, ys . all p (xs ++ ys) = all p xs ∧ all p ys

Theorem A : (x:xs) ++ ys = x:(xs ++ ys)

For all xs, ys:
    By induction on `xs`:
        Base case: xs = []
            all p ([] ++ ys) = all p [] ∧ all p ys
                <Definition of all, Identity of `and`>
            all p ([] ++ ys) = all p ys
                <Identity of `++`>
            all p (ys) = all p ys
                <Reflexivity of equality>
            True
        Induction step: xs = k:ks
            all p (k:ks ++ ys) = all p k:ks ∧ all p ys
                <Definition of all>
            all p (k:ks ++ ys) = (p k ∧ (all p ks)) ∧ all p ys
                <Theorem A>
            all p k:(ks ++ ys) = (p k ∧ (all p ks)) ∧ all p ys
                <Definition of all>
            p k ∧ (all p (ks ++ ys)) = (p k ∧ (all p ks)) ∧ all p ys
                <Induction hypothesis>
            p k ∧ (all p ks ∧ all p ys) = (p k ∧ (all p ks)) ∧ all p ys
                <Associativity of ∧,  Reflexivity of equality>
            True 

\begin{code}
--------------------Question7--------------------
mystery :: ((a, b) -> c) -> [a] -> [b] -> [c]
mystery _ [] _ = []
mystery _ _ [] = []
mystery f (x : xs) (y : ys) = f (x, y) : (mystery f xs ys) 

\end{code}

\begin{code}
--------------------Question8--------------------
--foldr :: (a -> b -> b) -> b -> [a] -> b
reverse' :: [a] -> [a]
reverse' [] = []
reverse' xs = foldr (\x y -> y ++ [x]) [] xs
\end{code}

Bonus:

Original reverse is defined as (per Haskell Documentation):
\begin{code}
reverse'' :: [a] -> [a]
reverse'' l =  rev'' l []
  where
    rev'' []     a = a
    rev'' (x:xs) a = rev'' xs (x:a)
\end{code}

Universal propery is defined as (per "A tutorial on the universality and expressiveness of fold"):
    g [ ] = v             
    g (x : xs) = f x (g xs)  <=>  g = fold f v

To calculate parameters of the required fold we must solve the following equation:
    
    reverse'' = fold f v

Therefore:
    reverse''
        =<Definition of reverse''>
    rev'' l []
        =<Universal property>

Rearranged equation:

    rev'' l [] = fold f v

    Taking 

        <Proving each pattern separately>
            Pattern `rev'' [] [] = fold f v`:
                <Universal property, Definition of rev''>
                    [] = []
                <Reflexivity of equality>
                    True
            Pattern `rev'' l:ls [] = fold f v`:
                <Definition of rev''>
                    rev'' ls l:[] = fold f v
                <Prepending empty list>
                    rev'' ls [l] = fold f v
                <
    
    rev'' [] [] = []
    rev'' (x:xs) [] = rev'' xs (x:[])
    
        <Simplifying definition of rev'', Prepending to empty list>

    rev'' [] [] = [] 
    rev'' (x:xs) [] = rev'' xs x
        
        <Taking second pattern and applying Definition of rev''>
    rev'' xs (x:a) = rev'' xs (x : v) 

Therefore via definition of rev'' modified with a flip and definition of universal property
    flip rev'' v     [] = v
    flip rev'' v (x:xs) = flip rev'' (x `f` v) xs


f = (\x y -> y ++ [x])  
v = []

reverse xs = foldr (\x y -> y ++ [x]) [] xs

%%%%%%%%%%%%%%%%%%%%%%%%%%%%%%%%%%%%%%%%%%%%%%%%%%%%%%%%%


\begin{code}
--------------------Question9--------------------
data Tree a = Tip | Node ( Tree a )  a  ( Tree a )

mirrorTree :: Tree a -> Tree a
mirrorTree  Tip = Tip
mirrorTree  (Node l a r) = Node (mirrorTree  r)  a  (mirrorTree  l)

pre :: Tree a -> [a]
pre Tip = []
pre (Node l a r) = a : ((pre l) ++ (pre r))

post :: Tree a -> [a]
post Tip = []
post (Node l a r) = ((post l) ++ (post r)) ++ [a]


\end{code}
Prove:
    pre (mirrorTree t) = reverse (post t)

Theorem A: reverse (a ++ b ++ c) = (reverse c) ++ (reverse b) ++ (reverse a)

By induction:
    Base case: t = Tip
        pre (mirrorTree Tip) = reverse (post Tip)
            <Definition of mirrorTree, Definition of post>
        pre (Tip) = reverse ([])
            <Definition of pre, Definition reverse>
        [] = []
            <Reflexivity of equality>
        True
    Induction step: t = Node x y z
        pre (mirrorTree (Node x y z) = reverse (post (Node x y z))
            <Definition of post>
        LHS = reverse ((post x) ++ (post z) ++ [y])
            <Theorem A>
        LHS = reverse [y] ++ reverse (post z) ++ reverse (post x)
            <Reverse of singleton, Induction hypothesis>
        LHS = [y] ++ pre (mirrorTree z) ++ pre (mirrorTree x)
            <Definition of pre>
        LHS = pre (Node (mirrorTree z) y (mirrorTree x))
            <Definition of mirrorTree>
        pre (mirrorTree (Node x y z) = pre (mirrorTree (Node x y z)
            <Reflexivity of equality>
        true

\begin{code}
--------------------Question10--------------------
data Rose a = Rose a [Rose a]
data Fork a = Leaf a | Branch (Fork a) (Fork a)

to' :: Tree a -> [Rose a]
to' Tip = []
to' (Node l n r) = [Rose n (to' l ++ to' r)]

from' :: [Rose a] -> Tree a
from' [] = Tip
from' ((Rose o i) : xs) = Node (from' i) o (from' xs)

to :: Rose a -> Fork a
to (Rose o []) = Leaf o
to (Rose o [x])  = Branch (to x) (Leaf o)
to (Rose o [x,y]) = Branch (to x) (Branch (to y) (Leaf o)) 

from :: Fork a -> Rose a
from (Leaf x)     = Rose x []
from (Branch x y) = rosePack ((\(node, roses) -> (node, ([from x] ++ roses))) (roseUnpack (from y)))

roseUnpack :: Rose a -> (a, [Rose a])
roseUnpack (Rose x ys) = (x, ys)

rosePack :: (a, [Rose a]) -> Rose a
rosePack (x, ys) = (Rose x ys)

\end{code}

Prove:
    ∀xs.to (from xs) = xs

For all xs:
    By induction on `xs`:
        Base case: xs = Leaf k
            to (from Leaf k) = Leaf k
                <Definition of from>
            to(Rose k []) = Leaf k
                <Definition of to>
            Leaf k  = Leaf k
                <Reflexivity of equality>
            True
        Induction step: xs = Branch (Fork k) (Fork m)
            to (from Branch (Fork k) (Fork m)) = Branch (Fork k) (Fork m)
                <Definition for from>
            to (rosePack ((\(node, roses) -> (node, ([from Fork k] ++ roses))) (roseUnpack (from Fork m)))) = RHS
                <Combining definition of rosePack with lambda function>
            to ((\(node, roses) -> Rose (node) ([from Fork k] ++ roses)) (roseUnpack (from Fork m))) = RHS
                <Combining definition of roseUnpack with lambda function>
            to ((\Rose node roses -> Rose (node) ([from Fork k] ++ roses)) (from Fork m)) = RHS
                <?>
            True